schorr-waite: towards an invariant
The state update condition doesn't reflect the modified links
on the path.

schorr-waite/GraphMark.thy
@@ -12,8 +12,8 @@ context graph_mark begin
 
 type_synonym state_pred = "lifted_globals \<Rightarrow> bool"
 
-definition ok :: "node_C ptr \<Rightarrow> state_pred" where
-  "ok p s \<equiv> p \<noteq> NULL \<and> is_valid_node_C s p"
+definition ptr_ok :: "node_C ptr \<Rightarrow> state_pred" where
+  "ptr_ok p s \<equiv> p \<noteq> NULL \<and> is_valid_node_C s p"
 
 definition out :: "lifted_globals \<Rightarrow> node_C ptr \<Rightarrow> node_C ptr set" where
   "out s p \<equiv> { s[p]\<rightarrow>left, s[p]\<rightarrow>right }"
@@ -21,30 +21,66 @@ definition out :: "lifted_globals \<Rightarrow> node_C ptr \<Rightarrow> node_C 
 definition mark :: "bool \<Rightarrow> node_C \<Rightarrow> node_C" where
   "mark c node \<equiv> if c then node \<lparr> mark_C := 3 \<rparr> else node"
 
-definition mark_precond :: "state_pred \<Rightarrow> node_C ptr \<Rightarrow> state_pred" where
-  "mark_precond P root \<equiv> \<lambda> s. let R = reach (out s) {root} in
-    (\<forall> p \<in> R. ok p s \<and> s[p]\<rightarrow>mark = 0) \<and> P (heap_node_C_update (\<lambda> h p. mark (p \<in> R) (h p)) s)"
+definition mark_precondition :: "state_pred \<Rightarrow> node_C ptr \<Rightarrow> state_pred" where
+  "mark_precondition P root \<equiv> \<lambda> s. let R = reach (out s) {root} in
+    (\<forall> p \<in> R. ptr_ok p s \<and> s[p]\<rightarrow>mark = 0) \<and> P (heap_node_C_update (\<lambda> h p. mark (p \<in> R) (h p)) s)"
 
 primrec roots :: "node_C ptr \<times> node_C ptr \<Rightarrow> node_C ptr set" where
   "roots (p,q) = { r \<in> {p,q}. r \<noteq> NULL }"
 
-primrec mark_path :: "state_pred \<Rightarrow> node_C ptr list \<Rightarrow> state_pred" where
-  "mark_path P [] s = True" |
-  "mark_path P (p # ps) s =
-    (s[p]\<rightarrow>mark = 1 \<and> True)"
+type_synonym path_ok_t =
+  "lifted_globals \<Rightarrow> lifted_globals \<Rightarrow> node_C ptr set
+    \<Rightarrow> node_C ptr \<Rightarrow> node_C ptr \<Rightarrow> node_C ptr \<Rightarrow> node_C ptr list \<Rightarrow> bool "
 
-primrec mark_invariant :: "state_pred \<Rightarrow> node_C ptr \<times> node_C ptr \<Rightarrow> state_pred" where
-  "mark_invariant P (p,q) s = (\<exists> path. mark_path P path s)"
+primrec tail_ok :: path_ok_t where
+  "tail_ok s t M r q p [] = (p = NULL \<and> q = r)" |
+  "tail_ok s t M r q p (p' # ps) =
+    (p = p' \<and>
+      ((t[p]\<rightarrow>mark = 1 \<and>
+          t[p]\<rightarrow>left = q \<and> t[p]\<rightarrow>right = s[p]\<rightarrow>left \<and> tail_ok s t M r p s[p]\<rightarrow>right ps) \<or>
+       (t[p]\<rightarrow>mark = 2 \<and> t[p]\<rightarrow>left \<in> M \<and>
+          t[p]\<rightarrow>right = q \<and> t[p]\<rightarrow>left = s[p]\<rightarrow>right \<and> tail_ok s t M r p s[p]\<rightarrow>left ps)))"
+
+primrec path_ok :: path_ok_t where
+  "path_ok s t M r q p [] = (p = NULL \<and> q = r)" |
+  "path_ok s t M r q p (p' # ps) =
+    (p = p' \<and>
+      ((t[p]\<rightarrow>mark = 0 \<and>
+          t[p]\<rightarrow>left = s[p]\<rightarrow>left \<and> t[p]\<rightarrow>right = s[p]\<rightarrow>right) \<or>
+       (t[p]\<rightarrow>mark = 1 \<and> t[p]\<rightarrow>left \<in> M \<and>
+          t[p]\<rightarrow>left = q \<and> t[p]\<rightarrow>right = s[p]\<rightarrow>left \<and> tail_ok s t M r p s[p]\<rightarrow>right ps) \<or>
+       (t[p]\<rightarrow>mark = 2 \<and> t[p]\<rightarrow>left \<in> M \<and> t[p]\<rightarrow>right \<in> M \<and>
+          t[p]\<rightarrow>right = q \<and> t[p]\<rightarrow>left = s[p]\<rightarrow>right \<and> tail_ok s t M r p s[p]\<rightarrow>left ps)))"
+
+primrec mark_invariant :: "state_pred \<Rightarrow> node_C ptr \<Rightarrow> node_C ptr \<times> node_C ptr \<Rightarrow> state_pred" where
+  "mark_invariant P root (p,q) s =
+    (\<exists> t path M.
+      let
+        R = reach (out t) {root};
+        U = R - M;
+        F = U - set path
+      in
+        P t \<and>
+        M = reach (out t) M \<and>
+        (\<forall> p \<in> R. ptr_ok p t) \<and>
+        (\<forall> p \<in> M. s[p]\<rightarrow>mark = 3) \<and>
+        (\<forall> p \<in> F. s[p]\<rightarrow>mark = 0) \<and>
+        path_ok s t M root q p path \<and>
+        R = reach (out s) (roots (p,q)) \<and>
+        t = heap_node_C_update (\<lambda> h p. mark (p \<in> U) (h p)) s)"
 
 primrec mark_measure :: "(node_C ptr \<times> node_C ptr) \<times> lifted_globals \<Rightarrow> nat" where
   "mark_measure (r,s) = setsum (\<lambda> p. 3 - unat s[p]\<rightarrow>mark) (reach (out s) (roots r))"
 
-lemma graph_mark'_correct: "\<lbrace> mark_precond P root \<rbrace> graph_mark' root \<lbrace> \<lambda> _. P \<rbrace>!"
+lemma graph_mark'_correct: "\<lbrace> mark_precondition P root \<rbrace> graph_mark' root \<lbrace> \<lambda> _. P \<rbrace>!"
   unfolding
-    graph_mark'_def mark_precond_def
-    whileLoop_add_inv[where I="mark_invariant P" and M="mark_measure"]
+    graph_mark'_def mark_precondition_def
+    whileLoop_add_inv[where I="mark_invariant P root" and M="mark_measure"]
   apply (wp; clarsimp)
-  sorry
+  subgoal for p q s t path M sorry
+  subgoal for q s t path M sorry
+  subgoal for s sorry
+  done
 
 end
 
